theories/TypeSyntax.v
@@ -1,5 +1,8 @@
 (** * Type syntax of mailbox types *)
 
+Require Import Classes.RelationClasses.
+Require Import Classes.Morphisms.
+
 From MailboxTypes Require Import Message.
 Open Scope mailbox_config_scope.
 
@@ -26,7 +29,7 @@ Inductive MPattern `{IMessage Message} : Type :=
 Fixpoint Pow (p : MPattern) (n : nat) : MPattern :=
   match n with
   | 0 => MPOne
-  | S n => MPChoice p (Pow p n)
+  | S n => MPComp p (Pow p n)
   end.
 
 (**
@@ -49,10 +52,15 @@ Definition MPEqual (e f : MPattern) : Prop :=
 
 Lemma MPZero_empty : forall m, ~ (valueOf m MPZero).
 Proof.
-  intros m.
-  destruct m.
+  intros m. destruct m;
   unfold not; intros valueOf; inversion valueOf.
 Qed.
+
+Lemma MPOne_EmptyMailbox : forall m, valueOf m MPOne -> m =ᵐᵇ EmptyMailbox.
+Proof.
+  intros m mIn. now inversion mIn.
+Qed.
+
 End MPattern_defs.
 
 (** Notation on mailbox pattern. Basically the same as in the paper. *)
@@ -66,6 +74,150 @@ Infix "⊙" := MPComp (at level 65, left associativity) : mailbox_pattern_scope.
 Notation "⋆ E" := (MPStar E) (at level 64) : mailbox_pattern_scope.
 Notation "« M »" := (MPMessage M) : mailbox_pattern_scope.
 Infix "∈" := valueOf (at level 67, left associativity) : mailbox_pattern_scope.
+Infix "≈" := MPEqual (at level 71, left associativity) : mailbox_pattern_scope.
+
+Section MPattern_props.
+
+Context `{MessageInterface : IMessage Message}.
+
+Example Example1 : ⟨⟩ ∈ (𝟙 ⊕ 𝟘).
+Proof.
+  apply MPValueChoiceLeft.
+  apply MPValueOne.
+Qed.
+
+Lemma MPInclusion_trans : forall e f g, MPInclusion e f -> MPInclusion f g -> MPInclusion e g.
+Proof.
+  intros e f g Inc1 Inc2.
+  unfold MPInclusion in *.
+  intuition.
+Qed.
+
+Lemma MPEqual_refl : forall e, e ≈ e.
+Proof.
+  intros.
+  unfold MPEqual.
+  split; unfold MPInclusion; easy.
+Qed.
+
+Lemma MPEqual_sym : forall e f, e ≈ f -> f ≈ e.
+Proof.
+  intros e f Eq.
+  unfold MPEqual in *.
+  intuition.
+Qed.
+
+Lemma MPEqual_trans : forall e f g, e ≈ f -> f ≈ g -> e ≈ g.
+Proof.
+  intros e f g Eq1 Eq2.
+  unfold MPEqual in *.
+  destruct Eq1 as [Eq1 Eq1'].
+  destruct Eq2 as [Eq2 Eq2'].
+  split; eapply MPInclusion_trans.
+  apply Eq1. apply Eq2.
+  apply Eq2'. apply Eq1'.
+Qed.
+
+Global Instance MPEqual_equiv : Equivalence MPEqual.
+Proof.
+  constructor.
+  - unfold Reflexive. apply MPEqual_refl.
+  - unfold Symmetric. apply MPEqual_sym.
+  - unfold Transitive. apply MPEqual_trans.
+Defined.
+
+Global Instance MPEqual_valueOf_Proper : Proper (eq ==> MPEqual ==> iff) valueOf.
+Proof.
+  intros m1 m2 mbEq mp1 mp2 mpEq.
+  subst.
+  split.
+  - intros mIn.
+    induction mIn; inversion mpEq as [Eq1 Eq2]; unfold MPInclusion in *; apply Eq1;
+    try (now constructor).
+    eapply MPValueComp. apply mIn1. apply mIn2. apply H.
+  - intros mIn.
+    induction mIn; inversion mpEq as [Eq1 Eq2]; unfold MPInclusion in *; apply Eq2;
+    try (now constructor).
+    eapply MPValueComp. apply mIn1. apply mIn2. apply H.
+Defined.
+
+Lemma mailbox_eq_valueOf : forall m1 m2 mp, m1 =ᵐᵇ m2 -> m1 ∈ mp -> m2 ∈ mp.
+Proof.
+  intros ? ? ? mbEq mIn.
+  induction mIn as [| | | | ? ? ? ? ? ? ? ? ? mbEq2 | ? ? pow].
+  (* TODO use lemma for empty mailbox *)
+  - unfold mailbox_eq in *;
+    apply Permutation.Permutation_nil in mbEq; subst; constructor.
+  - apply SingletonMailbox_eq in mbEq; subst; constructor.
+  - constructor; now apply IHmIn.
+  - apply MPValueChoiceRight; now apply IHmIn.
+  - eapply MPValueComp; try (apply mIn1 || apply mIn2).
+    etransitivity. symmetry. apply mbEq. apply mbEq2.
+  - constructor; destruct pow as [n mIn2]; exists n;
+    induction n; simpl in *;
+    inversion mIn2 as [| | | | ? ? ? ? ? mInA mInB mbEq2 |]; subst.
+    + (* TODO use lemma for empty mailbox *)
+      apply Permutation.Permutation_nil in mbEq. subst. constructor.
+    + eapply MPValueComp. apply mInA. apply mInB.
+      etransitivity. symmetry. apply mbEq. apply mbEq2.
+Qed.
+
+Global Instance mailbox_eq_valueOf_Proper : Proper (mailbox_eq ==> MPEqual ==> iff) valueOf.
+Proof.
+  intros m1 m2 mbEq mp1 mp2 mpEq.
+  split.
+  - intros mIn.
+    eapply mailbox_eq_valueOf.
+    apply mbEq.
+    now setoid_rewrite <- mpEq.
+  - intros.
+    eapply mailbox_eq_valueOf.
+    symmetry.
+    apply mbEq.
+    now setoid_rewrite mpEq.
+Qed.
+
+Lemma MPChoice_unit : forall e, e ⊕ 𝟘 ≈ e.
+Proof.
+  intros e.
+  unfold MPEqual; split; unfold MPInclusion; intros m mIn.
+  - now inversion mIn.
+  - now constructor.
+Qed.
+
+Lemma MPComp_unit : forall e, e ⊙ 𝟙 ≈ e.
+Proof.
+  intros e.
+  unfold MPEqual; split; unfold MPInclusion; intros m mIn.
+  - inversion mIn; subst. apply MPOne_EmptyMailbox in H3.
+    setoid_rewrite H3 in H4.
+    rewrite mailbox_union_comm in H4.
+    rewrite <- mailbox_union_empty_left in H4.
+    now setoid_rewrite H4.
+  - inversion mIn; subst;
+    try (apply MPValueComp with (a := nil) (b := nil); constructor; constructor);
+    try (apply MPValueComp with (a := ⟨ m0 ⟩) (b := nil);
+        constructor; constructor; reflexivity);
+    try ( apply MPValueComp with (a := m) (b := nil);
+        try (apply mIn || constructor);
+             unfold mailbox_union; now rewrite List.app_nil_r
+    ).
+Qed.
+
+(* TODO *)
+(*
+Lemma MPComp_assoc : forall e f g, e ⊙ (f ⊙ g) ≈ (e ⊙ f) ⊙ g.
+Proof.
+  intros e f g.
+  unfold MPEqual.
+  split.
+  - unfold MPInclusion.
+    intros m mIn.
+    destruct e; destruct f; destruct g.
+    + simpl.
+*)
+
+End MPattern_props.
 
 Require Import String.
 Open Scope string_scope.
